Stable, begin proving beta conv

Beta.v
@@ -1440,3 +1440,1921 @@ Proof.
     eapply compare_branches_forall; tauto.
 Qed.
 
+
+
+
+Definition valptr := nat.
+Definition rthreadptr := nat.
+Definition cthreadptr := nat.
+Definition threadptr := (nat + nat)%type.
+
+Definition varname := nat.
+
+Definition env := list valptr.
+
+Inductive cont :=
+| Kid : cont
+| Kapp : valptr -> cont -> cont
+| Kswitch : list (nat * term) -> env -> list (list varname * valptr) -> cont -> cont.
+
+Record neutral := mkneutral {
+  n_id : varname ;
+  n_cont : cont ;
+  n_unfold : option valptr ;
+}.
+
+Inductive value :=
+| Thread : rthreadptr -> value
+| Neutral : neutral -> value
+| Clos : term -> env -> varname -> valptr -> value
+| Block : nat -> list valptr -> value.
+
+Inductive code :=
+| Term : term -> env -> code
+| Val : valptr -> code.
+
+Record rthread := mkrthread {
+  rt_code : code ;
+  rt_cont : cont ;
+}.
+
+
+
+Inductive addr :=
+| a_rthread : rthreadptr -> addr
+| a_val : valptr -> addr.
+
+Definition env_points_to e a :=
+  match a with
+  | a_val vp => In vp e
+  | _ => False
+  end.
+
+Inductive cont_points_to : cont -> addr -> Prop :=
+| kapp_points_to_1 : forall vp c, cont_points_to (Kapp vp c) (a_val vp)
+| kapp_points_to_2 : forall vp c a, cont_points_to c a -> cont_points_to (Kapp vp c) a
+| kswitch_points_to_1 : forall bs e bds c a, env_points_to e a -> cont_points_to (Kswitch bs e bds c) a
+| kswitch_points_to_2 : forall bs e bds c a, cont_points_to c a -> cont_points_to (Kswitch bs e bds c) a.
+
+Inductive val_points_to : value -> addr -> Prop :=
+| thread_points_to : forall rid, val_points_to (Thread rid) (a_rthread rid)
+| neutral_points_to_1 : forall n a, cont_points_to n.(n_cont) a -> val_points_to (Neutral n) a
+(* todo | neutral_points_to_2 : *)
+| clos_points_to_1 : forall t e vn vp a, env_points_to e a -> val_points_to (Clos t e vn vp) a
+| clos_points_to_2 : forall t e vn vp, val_points_to (Clos t e vn vp) (a_val vp)
+| block_points_to : forall tag l a, env_points_to l a -> val_points_to (Block tag l) a.
+
+Inductive code_points_to : code -> addr -> Prop :=
+| term_points_to : forall t e a, env_points_to e a -> code_points_to (Term t e) a
+| cval_points_to : forall vp, code_points_to (Val vp) (a_val vp).
+
+Definition rthread_points_to rt a := code_points_to rt.(rt_code) a \/ cont_points_to rt.(rt_cont) a.
+
+Definition points_to rthreads vals a1 a2 :=
+  match a1 with
+  | a_rthread rid =>
+    match nth_error rthreads rid with
+    | Some rt => rthread_points_to rt a2
+    | None => False
+    end
+  | a_val vp =>
+    match nth_error vals vp with
+    | Some v => val_points_to v a2
+    | None => False
+    end
+  end.
+
+Definition valid (rthreads : list rthread) (vals : list value) a :=
+  match a with
+  | a_rthread rid => rid < length rthreads
+  | a_val vp => vp < length vals
+  end.
+
+Definition valid_addrs rthreads vals :=
+  forall a1 a2, points_to rthreads vals a1 a2 -> valid rthreads vals a2.
+
+Definition state_ok rthreads vals := well_founded (flip (points_to rthreads vals)) /\ valid_addrs rthreads vals.
+
+Record state := mkstate {
+  st_rthreads : list rthread ;
+  st_vals : list value ;
+  st_freename : nat ;
+(*  st_ok : state_ok st_rthreads st_vals ; *)
+}.
+
+Fixpoint update {A : Type} (l : list A) (k : nat) (x : A) : list A :=
+  match l with
+  | nil => nil
+  | y :: l =>
+    match k with
+    | O => x :: l
+    | S k => y :: update l k x
+    end
+  end.
+Arguments update {A} _ _ _ : simpl nomatch.
+
+Inductive plus {A : Type} (R : A -> A -> Prop) : A -> A -> Prop :=
+| plus_1 : forall x y, R x y -> plus R x y
+| plus_S : forall x y z, R x y -> plus R y z -> plus R x z.
+
+Lemma nth_error_update :
+  forall (A : Type) (l : list A) k x y, nth_error l k = Some x -> nth_error (update l k y) k = Some y.
+Proof.
+  induction l; intros [|k] x y; simpl in *; intros; try congruence.
+  eapply IHl; eassumption.
+Qed.
+
+Lemma nth_error_update2 :
+  forall (A : Type) (l : list A) k x, nth_error (update l k x) k = match nth_error l k with Some _ => Some x | None => None end.
+Proof.
+  induction l; intros [|k] x; simpl in *; intros; try congruence.
+  apply IHl.
+Qed.
+
+Lemma nth_error_update3 :
+  forall (A : Type) (l : list A) k1 k2 x, k1 <> k2 -> nth_error (update l k1 x) k2 = nth_error l k2.
+Proof.
+  induction l; intros [|k1] [|k2] x H; simpl in *; try congruence.
+  apply IHl; congruence.
+Qed.
+
+Lemma plus_star :
+  forall (A : Type) (R : A -> A -> Prop) x y, plus R x y -> star R x y.
+Proof.
+  intros A R x y H; induction H.
+  - apply star_1. assumption.
+  - econstructor; eassumption.
+Qed.
+
+Lemma plus_star_iff :
+  forall (A : Type) (R : A -> A -> Prop) x y, plus R x y <-> compose R (star R) x y.
+Proof.
+  intros A R x y; split; intros H.
+  - inversion H; subst.
+    + exists y; split; [assumption|apply star_refl].
+    + exists y0. split; [assumption|apply plus_star; assumption].
+  - destruct H as (z & Hxz & Hzy).
+    revert x Hxz; induction Hzy; intros w Hw.
+    + apply plus_1; assumption.
+    + eapply plus_S; [eassumption|apply IHHzy; assumption].
+Qed.
+
+Lemma Acc_star_down :
+  forall (A : Type) (R : A -> A -> Prop) x y, Acc R x -> star R y x -> Acc R y.
+Proof.
+  intros A R x y H1 H2. induction H2.
+  - assumption.
+  - apply IHstar in H1. inversion H1.
+    apply H0. assumption.
+Qed.
+
+Lemma plus_compose_star_left :
+  forall (A : Type) (R : A -> A -> Prop) x y z, star R x y -> plus R y z -> plus R x z.
+Proof.
+  intros A R x y z H1 H2; induction H1; [assumption|].
+  econstructor; [eassumption|].
+  apply IHstar; assumption.
+Qed.
+
+Lemma flip_plus :
+  forall (A : Type) (R : A -> A -> Prop) x y, plus (flip R) x y -> plus R y x.
+Proof.
+  intros A R x y H. induction H.
+  - apply plus_1. assumption.
+  - eapply plus_compose_star_left; [eapply plus_star; eassumption|].
+    apply plus_1. assumption.
+Qed.
+
+Lemma plus_same_rel :
+  forall (A : Type) (R1 R2 : A -> A -> Prop), same_rel R1 R2 -> same_rel (plus R1) (plus R2).
+Proof.
+  intros A R1 R2 H x y. split; intros Hplus; induction Hplus.
+  - apply plus_1, H. assumption.
+  - eapply plus_S; [|eassumption]. apply H. assumption.
+  - apply plus_1, H. assumption.
+  - eapply plus_S; [|eassumption]. apply H. assumption.
+Qed.
+
+Lemma flip_flip :
+  forall (A : Type) (R : A -> A -> Prop), same_rel (flip (flip R)) R.
+Proof.
+  intros A R x y. reflexivity.
+Qed.
+
+Lemma flip_plus_iff :
+  forall (A : Type) (R : A -> A -> Prop) x y, plus (flip R) x y <-> plus R y x.
+Proof.
+  intros A R x y; split; intros H.
+  - apply flip_plus. assumption.
+  - eapply flip_plus, plus_same_rel; [|eassumption].
+    apply flip_flip.
+Qed.
+
+Lemma plus_compose_star_right :
+  forall (A : Type) (R : A -> A -> Prop) x y z, plus R x y -> star R y z -> plus R x z.
+Proof.
+  intros A R x y z H1 H2.
+  apply flip_plus_iff.
+  eapply plus_compose_star_left; [|apply flip_plus_iff; eassumption].
+  apply star_flip in H2. eassumption.
+Qed.
+
+Lemma Acc_plus :
+  forall (A : Type) (R : A -> A -> Prop) x, Acc R x -> Acc (plus R) x.
+Proof.
+  intros A R x H. induction H.
+  constructor. intros y Hy.
+  apply flip_plus_iff in Hy.
+  inversion Hy; subst.
+  - apply H0. assumption.
+  - eapply Acc_star_down; [eapply H0; eassumption|].
+    apply star_1, flip_plus_iff; eassumption.
+Qed.
+
+Definition updatep {A B : Type} (f : A -> B -> Prop) (x : A) (P : B -> Prop) (u : A) (v : B) :=
+  (u <> x /\ f u v) \/ (u = x /\ P v).
+
+(*
+Lemma updatep_wf :
+  forall (A : Type) (R : A -> A -> Prop) u (P : A -> Prop),
+    (forall v, P v -> plus R u v) -> well_founded R -> well_founded (updatep R u P).
+Proof.
+  intros A R u P H Hwf v.
+  induction (Acc_plus _ _ _ (Hwf v)). constructor.
+  intros v [[Huv HR] | [-> HP]].
+  - apply H1, plus_1, HR.
+  - apply H1, H, HP.
+Qed.
+*)
+
+(*
+Lemma updatep_wf :
+  forall (A : Type) (R : A -> A -> Prop) u (P : A -> Prop),
+    (forall v, P v -> plus R u v \/ Acc (flip (updatep R u P)) v) -> well_founded (flip R) -> well_founded (flip (updatep R u P)).
+Proof.
+  intros A R u P H Hwf v.
+  induction (Acc_plus _ _ _ (Hwf v)). constructor.
+  intros v [[Huv HR] | [-> HP]].
+  - apply H1, plus_1, HR.
+  - destruct (H _ HP) as [Hplus | Hacc]; [apply H1, flip_plus_iff, Hplus|apply Hacc].
+Qed.
+*)
+
+Inductive AccI {A : Type} (B : A -> Prop) (R : A -> A -> Prop) : A -> Prop :=
+| AccI_base : forall a, B a -> AccI B R a
+| AccI_intro : forall a, (forall b, R b a -> AccI B R b) -> AccI B R a.
+
+Lemma updatep_wf2 :
+  forall (A : Type) (R : A -> A -> Prop) u (P : A -> Prop),
+    (forall v, P v -> AccI (fun v => plus R u v) (flip (updatep R u P)) v) -> well_founded (flip R) -> well_founded (flip (updatep R u P)).
+Proof.
+  intros A R u P H Hwf v.
+  induction (Acc_plus _ _ _ (Hwf v)). constructor.
+  intros v [[Huv HR] | [-> HP]].
+  - apply H1, plus_1, HR.
+  - specialize (H _ HP). clear HP. induction H.
+    + apply H1, flip_plus_iff, H.
+    + constructor. apply H2.
+Qed.
+
+Lemma updatep_wf_none :
+  forall (A : Type) (R : A -> A -> Prop) u (P : A -> Prop),
+    ~ P u -> (forall v, ~ R v u) -> well_founded (flip R) -> well_founded (flip (updatep R u P)).
+Proof.
+  intros A R u P HP Hu Hwf.
+  assert (Hwf1 : forall v, v <> u -> Acc (flip (updatep R u P)) v).
+  - intros v Hv. induction (Hwf v). constructor.
+    intros v [[Huv HR] | [-> HPv]].
+    + apply H0; [assumption|]. intros ->; eapply Hu, HR.
+    + tauto.
+  - intros v. constructor; intros w [[Hvw HR2] | [-> HPw]].
+    + apply Hwf1. intros ->; eapply Hu, HR2.
+    + apply Hwf1. intros ->; apply HP, HPw.
+Qed.
+
+Lemma Acc_ext :
+  forall (A : Type) (R1 R2 : A -> A -> Prop) x, (forall u v, R2 u v -> R1 u v) -> Acc R1 x -> Acc R2 x.
+Proof.
+  intros A R1 R2 x H Hwf; induction Hwf; constructor.
+  intros y HR; apply H1, H, HR.
+Qed.
+
+Lemma AccI_ext :
+  forall (A : Type) (B : A -> Prop) (R1 R2 : A -> A -> Prop) x, (forall u v, R2 u v -> R1 u v) -> AccI B R1 x -> AccI B R2 x.
+Proof.
+  intros A B R1 R2 x H Hwf; induction Hwf.
+  - apply AccI_base; assumption.
+  - apply AccI_intro; intros; apply H1, H, H2.
+Qed.
+
+Lemma well_founded_ext :
+  forall (A : Type) (R1 R2 : A -> A -> Prop), (forall u v, R2 u v -> R1 u v) -> well_founded R1 -> well_founded R2.
+Proof.
+  intros A R1 R2 H Hwf x; eapply Acc_ext; [eassumption|apply Hwf].
+Qed.
+
+
+
+Lemma points_to_updatep_rthread :
+  forall rthreads vals rid rt a1 a2,
+    points_to (update rthreads rid rt) vals a1 a2 <->
+    updatep (points_to rthreads vals) (a_rthread rid) (fun a => rid < length rthreads /\ rthread_points_to rt a) a1 a2.
+Proof.
+  intros rthreads vals rid rt [rid2|vp] a; unfold updatep; simpl; [|intuition congruence].
+  destruct (Nat.eq_dec rid rid2); subst.
+  - rewrite nth_error_update2.
+    destruct nth_error eqn:Hnth; [apply nth_error_Some3 in Hnth|apply nth_error_None in Hnth]; intuition lia.
+  - rewrite nth_error_update3; [|assumption].
+    intuition congruence.
+Qed.
+
+Lemma points_to_updatep_vals :
+  forall rthreads vals vp v a1 a2,
+    points_to rthreads (update vals vp v) a1 a2 <->
+    updatep (points_to rthreads vals) (a_val vp) (fun a => vp < length vals /\ val_points_to v a) a1 a2.
+Proof.
+  intros rthreads vals vp v [rid|vp2] a; unfold updatep; simpl; [intuition congruence|].
+  destruct (Nat.eq_dec vp vp2); subst.
+  - rewrite nth_error_update2.
+    destruct nth_error eqn:Hnth; [apply nth_error_Some3 in Hnth|apply nth_error_None in Hnth]; intuition lia.
+  - rewrite nth_error_update3; [|assumption].
+    intuition congruence.
+Qed.
+
+Lemma points_to_updatep_rthread_extend :
+  forall rthreads vals rt a1 a2,
+    points_to (rthreads ++ rt :: nil) vals a1 a2 <->
+    updatep (points_to rthreads vals) (a_rthread (length rthreads)) (rthread_points_to rt) a1 a2.
+Proof.
+  intros rthreads vals rt [rid|vp] a; unfold updatep; simpl; [|intuition congruence].
+  destruct (le_lt_dec (length rthreads) rid).
+  - rewrite nth_error_app2 by assumption.
+    remember (rid - length rthreads) as n. destruct n as [|m] eqn:Hn.
+    + simpl. assert (rid = length rthreads) by lia. intuition congruence.
+    + simpl. do 2 (replace (nth_error _ _) with (@None rthread) by (symmetry; apply nth_error_None; simpl; lia)).
+      assert (rid <> length rthreads) by lia. intuition congruence.
+  - rewrite nth_error_app1 by assumption.
+    assert (rid <> length rthreads) by lia.
+    destruct nth_error; intuition congruence.
+Qed.
+
+Lemma points_to_updatep_val_extend :
+  forall rthreads vals v a1 a2,
+    points_to rthreads (vals ++ v :: nil) a1 a2 <->
+    updatep (points_to rthreads vals) (a_val (length vals)) (val_points_to v) a1 a2.
+Proof.
+  intros rthreads vals v [rid|vp] a; unfold updatep; simpl; [intuition congruence|].
+  destruct (le_lt_dec (length vals) vp).
+  - rewrite nth_error_app2 by assumption.
+    remember (vp - length vals) as n. destruct n as [|m] eqn:Hn.
+    + simpl. assert (vp = length vals) by lia. intuition congruence.
+    + simpl. do 2 (replace (nth_error _ _) with (@None value) by (symmetry; apply nth_error_None; simpl; lia)).
+      assert (vp <> length vals) by lia. intuition congruence.
+  - rewrite nth_error_app1 by assumption.
+    assert (vp <> length vals) by lia.
+    destruct nth_error; intuition congruence.
+Qed.
+
+
+
+
+Lemma update_length :
+  forall {A : Type} (l : list A) k x, length (update l k x) = length l.
+Proof.
+  induction l; intros [|k] x; simpl in *; congruence.
+Qed.
+
+Definition update_rthread_hyp rthreads vals rid rt :=
+  forall a, rthread_points_to rt a -> AccI (plus (points_to rthreads vals) (a_rthread rid)) (flip (points_to (update rthreads rid rt) vals)) a /\ valid rthreads vals a.
+
+Lemma update_rthread_wf :
+  forall rthreads vals rid rt,
+    update_rthread_hyp rthreads vals rid rt ->
+     well_founded (flip (points_to rthreads vals)) -> well_founded (flip (points_to (update rthreads rid rt) vals)).
+Proof.
+  intros rthreads vals rid rt H Hwf.
+  eapply well_founded_ext; [|apply updatep_wf2; [|eassumption]].
+  - intros. apply points_to_updatep_rthread; eassumption.
+  - intros a [Hrid Ha].
+    eapply AccI_ext; [|eapply H; eassumption].
+    intros; apply points_to_updatep_rthread; eassumption.
+Qed.
+
+Lemma update_rthread_valid :
+  forall rthreads vals rid rt,
+    update_rthread_hyp rthreads vals rid rt ->
+    valid_addrs rthreads vals -> valid_addrs (update rthreads rid rt) vals.
+Proof.
+  intros rthreads vals rid rt H Hvalid [rid2|vp] a2 Ha; simpl in *; unfold valid.
+  - destruct (Nat.eq_dec rid rid2); subst.
+    + rewrite nth_error_update2 in Ha.
+      destruct nth_error eqn:Hrid2; [|tauto].
+      rewrite update_length.
+      apply H; assumption.
+    + rewrite nth_error_update3 in Ha by assumption.
+      rewrite update_length.
+      apply Hvalid with (a1 := a_rthread rid2); assumption.
+  - rewrite update_length.
+    apply Hvalid with (a1 := a_val vp); assumption.
+Qed.
+
+Lemma update_rthread_ok :
+  forall rthreads vals rid rt,
+    update_rthread_hyp rthreads vals rid rt ->
+    state_ok rthreads vals -> state_ok (update rthreads rid rt) vals.
+Proof.
+  intros rthreads vals rid rt H [Hwf Hvalid].
+  split; [apply update_rthread_wf|apply update_rthread_valid]; assumption.
+Qed.
+
+Definition update_val_hyp rthreads vals vp v :=
+  forall a, val_points_to v a -> AccI (plus (points_to rthreads vals) (a_val vp)) (flip (points_to rthreads (update vals vp v))) a /\ valid rthreads vals a.
+
+Lemma update_val_wf :
+  forall rthreads vals vp v,
+    update_val_hyp rthreads vals vp v ->
+     well_founded (flip (points_to rthreads vals)) -> well_founded (flip (points_to rthreads (update vals vp v))).
+Proof.
+  intros rthreads vals vp v H Hwf.
+  eapply well_founded_ext; [|apply updatep_wf2; [|eassumption]].
+  - intros. apply points_to_updatep_vals; eassumption.
+  - intros a [Hrid Ha].
+    eapply AccI_ext; [|eapply H; eassumption].
+    intros; apply points_to_updatep_vals; eassumption.
+Qed.
+
+Lemma update_val_valid :
+  forall rthreads vals vp v,
+    update_val_hyp rthreads vals vp v ->
+    valid_addrs rthreads vals -> valid_addrs rthreads (update vals vp v).
+Proof.
+  intros rthreads vals vp v H Hvalid [rid|vp2] a2 Ha; simpl in *; unfold valid.
+  - rewrite update_length.
+    apply Hvalid with (a1 := a_rthread rid); assumption.
+  - destruct (Nat.eq_dec vp vp2); subst.
+    + rewrite nth_error_update2 in Ha.
+      destruct nth_error eqn:Hvp2; [|tauto].
+      rewrite update_length.
+      apply H; assumption.
+    + rewrite nth_error_update3 in Ha by assumption.
+      rewrite update_length.
+      apply Hvalid with (a1 := a_val vp2); assumption.
+Qed.
+
+Lemma update_val_ok :
+  forall rthreads vals vp v,
+    update_val_hyp rthreads vals vp v ->
+    state_ok rthreads vals -> state_ok rthreads (update vals vp v).
+Proof.
+  intros rthreads vals vp v H [Hwf Hvalid].
+  split; [apply update_val_wf|apply update_val_valid]; assumption.
+Qed.
+
+Definition add_rthread_hyp rthreads vals rt :=
+  forall a, rthread_points_to rt a -> valid rthreads vals a.
+
+Lemma add_rthread_wf :
+  forall rthreads vals rt,
+    add_rthread_hyp rthreads vals rt ->
+    well_founded (flip (points_to rthreads vals)) ->
+    valid_addrs rthreads vals ->
+    well_founded (flip (points_to (rthreads ++ rt :: nil) vals)).
+Proof.
+  intros rthreads vals rt H Hwf Hvalid.
+  eapply well_founded_ext; [|apply updatep_wf_none; [| |eassumption]].
+  - intros. apply points_to_updatep_rthread_extend; eassumption.
+  - intros Hrt. apply H in Hrt; simpl in Hrt. lia.
+  - intros a Ha. apply Hvalid in Ha. simpl in Ha. lia.
+Qed.
+
+Lemma add_rthread_valid :
+  forall rthreads vals rt,
+    add_rthread_hyp rthreads vals rt ->
+    valid_addrs rthreads vals ->
+    valid_addrs (rthreads ++ rt :: nil) vals.
+Proof.
+  intros rthreads vals rt H Hvalid [rid|vp] a2 Ha; simpl in *; unfold valid; rewrite app_length; simpl.
+  - destruct (le_lt_dec (length rthreads) rid).
+    + rewrite nth_error_app2 in Ha by assumption.
+      destruct (rid - length rthreads) as [|n]; simpl in *; [|destruct n; simpl in *; tauto].
+      apply H in Ha. destruct a2; simpl in *; lia.
+    + rewrite nth_error_app1 in Ha by assumption.
+      apply (Hvalid (a_rthread rid)) in Ha.
+      destruct a2; simpl in *; lia.
+  - apply (Hvalid (a_val vp)) in Ha.
+    destruct a2; simpl in *; lia.
+Qed.
+
+Lemma add_rthread_ok :
+  forall rthreads vals rt,
+    add_rthread_hyp rthreads vals rt ->
+    state_ok rthreads vals -> state_ok (rthreads ++ rt :: nil) vals.
+Proof.
+  intros rthreads vals rt H [Hwf Hvalid].
+  split; [apply add_rthread_wf|apply add_rthread_valid]; assumption.
+Qed.
+
+
+Definition add_val_hyp rthreads vals v :=
+  forall a, val_points_to v a -> valid rthreads vals a.
+
+Lemma add_val_wf :
+  forall rthreads vals v,
+    add_val_hyp rthreads vals v ->
+    well_founded (flip (points_to rthreads vals)) ->
+    valid_addrs rthreads vals ->
+    well_founded (flip (points_to rthreads (vals ++ v :: nil))).
+Proof.
+  intros rthreads vals v H Hwf Hvalid.
+  eapply well_founded_ext; [|apply updatep_wf_none; [| |eassumption]].
+  - intros. apply points_to_updatep_val_extend; eassumption.
+  - intros Hv. apply H in Hv; simpl in Hv. lia.
+  - intros a Ha. apply Hvalid in Ha. simpl in Ha. lia.
+Qed.
+
+Lemma add_val_valid :
+  forall rthreads vals v,
+    add_val_hyp rthreads vals v ->
+    valid_addrs rthreads vals ->
+    valid_addrs rthreads (vals ++ v :: nil).
+Proof.
+  intros rthreads vals v H Hvalid [rid|vp] a2 Ha; simpl in *; unfold valid; rewrite app_length; simpl.
+  - apply (Hvalid (a_rthread rid)) in Ha.
+    destruct a2; simpl in *; lia.
+  - destruct (le_lt_dec (length vals) vp).
+    + rewrite nth_error_app2 in Ha by assumption.
+      destruct (vp - length vals) as [|n]; simpl in *; [|destruct n; simpl in *; tauto].
+      apply H in Ha. destruct a2; simpl in *; lia.
+    + rewrite nth_error_app1 in Ha by assumption.
+      apply (Hvalid (a_val vp)) in Ha.
+      destruct a2; simpl in *; lia.
+Qed.
+
+Lemma add_val_ok :
+  forall rthreads vals v,
+    add_val_hyp rthreads vals v ->
+    state_ok rthreads vals -> state_ok rthreads (vals ++ v :: nil).
+Proof.
+  intros rthreads vals v H [Hwf Hvalid].
+  split; [apply add_val_wf|apply add_val_valid]; assumption.
+Qed.
+
+
+Definition update_addr st a (v : match a return Type with a_rthread _ => rthread | a_val _ => value end) :=
+  match a, v with
+  | a_rthread rid, rt =>
+    {|
+      st_rthreads := update st.(st_rthreads) rid rt ;
+      st_vals := st.(st_vals) ;
+      st_freename := st.(st_freename) ;
+    |}
+  | a_val vp, v =>
+    {|
+      st_rthreads := st.(st_rthreads);
+      st_vals := update st.(st_vals) vp v ;
+      st_freename := st.(st_freename) ;
+    |}
+  end.
+
+Definition get_addr st a : option (match a return Type with a_rthread _ => rthread | a_val _ => value end) :=
+  match a with
+  | a_rthread rid => nth_error st.(st_rthreads) rid
+  | a_val vp => nth_error st.(st_vals) vp
+  end.
+
+Definition update_rthread st rid rt (* H *) :=
+(*  {|
+    st_rthreads := update st.(st_rthreads) rid rt ;
+    st_vals := st.(st_vals) ;
+    st_freename := st.(st_freename) ;
+(*    st_ok := update_rthread_ok _ _ _ _ H st.(st_ok) ; *)
+  |}. *)
+  update_addr st (a_rthread rid) rt.
+
+Lemma freevar_ok :
+  forall name rthreads vals,
+    state_ok rthreads vals -> state_ok rthreads (vals ++ Neutral {| n_id := name ; n_cont := Kid ; n_unfold := None |} :: nil).
+Proof.
+  intros name rthreads vals Hok.
+  apply add_val_ok; [|assumption].
+  intros a Ha; inversion Ha; subst.
+  inversion H0.
+Qed.
+
+Definition freevar (st : state) :=
+  ({|
+      st_rthreads := st.(st_rthreads) ;
+      st_vals := st.(st_vals) ++ Neutral {| n_id := st.(st_freename) ; n_cont := Kid ; n_unfold := None |} :: nil ;
+      st_freename := S st.(st_freename) ;
+      (* st_ok := freevar_ok _ _ _ st.(st_ok) ; *)
+    |}, st.(st_freename), length st.(st_vals)).
+
+Definition makelazy_hyp rthreads vals e :=
+  forall a, env_points_to e a -> valid rthreads vals a.
+
+Lemma makelazy_ok :
+  forall rthreads vals t e,
+    makelazy_hyp rthreads vals e ->
+    state_ok rthreads vals ->
+    state_ok (rthreads ++ {| rt_code := Term t e; rt_cont := Kid |} :: nil) (vals ++ Thread (length rthreads) :: nil).
+Proof.
+  intros rthreads vals t e Hmakelazy Hok.
+  eapply add_rthread_ok in Hok; [eapply add_val_ok; [|eassumption]|].
+  - intros a Ha. inversion Ha; subst. simpl.
+    rewrite app_length; simpl. lia.
+  - intros a Ha. inversion Ha; subst; inversion H; subst.
+    eapply Hmakelazy; eassumption.
+Qed.
+
+Definition makelazy (st : state) (t : term) (e : env) (* H *) :=
+  (* For now, ignore variable optimization *)
+  ({|
+    st_rthreads := st.(st_rthreads) ++ {| rt_code := Term t e ; rt_cont := Kid |} :: nil ;
+    st_vals := st.(st_vals) ++ Thread (length st.(st_rthreads)) :: nil ;
+    st_freename := st.(st_freename) ;
+    (* st_ok := makelazy_ok st.(st_rthreads) st.(st_vals) t e H st.(st_ok) ; *)
+    |}, length st.(st_vals)).
+
+
+(*
+Definition dummy_term := abs (var 0).
+
+Program Fixpoint read_thread st rid (acc : Acc (flip (points_to st.(st_rthreads) st.(st_vals))) (a_rthread rid)) {struct acc} :=
+  match acc with
+  | Acc_intro _ Hrec =>
+    match nth_error st.(st_rthreads) rid with
+    | None => dummy_term
+    | Some rt =>
+      let h := read_cont st rt.(rt_cont) _ in
+      match rt.(rt_code) with
+      | Val vp => read_val st vp (Hrec (a_val vp) _)
+      | Term t e => dummy_term (* todo *)
+      end
+    end
+  end
+
+with read_val st vp (acc : Acc (flip (points_to st.(st_rthreads) st.(st_vals))) (a_val vp)) {struct acc} :=
+  match acc with
+  | Acc_intro _ Hrec =>
+    match nth_error st.(st_vals) vp with
+    | None => dummy_term
+    | Some (Thread rid) => read_thread st rid (Hrec (a_rthread rid) _)
+    | Some (Clos t e x vp2) =>
+      dummy_term
+    | Some _ => dummy_term
+    end
+  end
+
+with read_cont st c (acc : forall a, cont_points_to c a -> Acc (flip (points_to st.(st_rthreads) st.(st_vals))) a) {struct c} :=
+  match c with
+  | Kid => h_hole
+  | Kapp vp c => h_app (read_cont st c _) (read_val st vp  _)
+  | Kswitch _ _ _ _ => h_hole
+  end.
+Next Obligation.
+  apply acc. apply kapp_points_to_2. assumption.
+Defined.
+Next Obligation.
+  apply acc. apply kapp_points_to_1.
+Defined.
+Next Obligation.
+  apply Hrec. unfold flip, points_to; simpl.
+  rewrite <- Heq_anonymous. right. assumption.
+Defined.
+Next Obligation.
+  unfold flip, points_to. rewrite <- Heq_anonymous0.
+  left. rewrite <- Heq_anonymous. constructor.
+Defined.
+Next Obligation.
+  unfold flip, points_to. rewrite <- Heq_anonymous.
+  constructor.
+Defined.
+Next Obligation.
+  split; intros; discriminate.
+Defined.
+Next Obligation.
+  split; intros; discriminate.
+Defined.
+
+Print read_thread.
+
+| read_thread_val : forall rid vp c t h,
+    nth_error st.(st_rthreads) rid = Some {| rt_code := Val vp ; rt_cont := c |} ->
+    read_val st vp t ->
+    read_cont st c h ->
+    read_thread st rid (fill_hctx h t)
+| read_thread_term : forall rid e el c t h,
+    nth_error st.(st_rthreads) rid = Some {| rt_code := Term t e ; rt_cont := c |} ->
+    Forall2 (read_val st) e el ->
+    read_cont st c h ->
+    read_thread st rid (fill_hctx h (subst (read_env el) t))
+
+with read_val st : valptr -> term -> Prop :=
+| read_val_thread :
+    forall vp rid t,
+      nth_error st.(st_vals) vp = Some (Thread rid) ->
+      read_thread st rid t ->
+      read_val st vp t
+| read_val_clos :
+    forall vp t e el x vp2,
+      nth_error st.(st_vals) vp = Some (Clos t e x vp2) ->
+      Forall2 (read_val st) e el ->
+      read_val st vp (subst (read_env el) (abs t))
+
+with read_cont st : cont -> hctx -> Prop :=
+| read_cont_kid : read_cont st Kid h_hole
+| read_cont_kapp :
+    forall vp c t h,
+      read_val st vp t ->
+      read_cont st c h ->
+      read_cont st (Kapp vp c) (h_app h t)
+| read_cont_kswitch :
+    forall bs e bds c el h,
+      Forall2 (read_val st) e el ->
+      read_cont st c h ->
+      read_cont st (Kswitch bs e bds c) (h_switch h (map (fun '(p, t) => (p, subst (read_env el) t)) bs)).
+
+*)
+
+
+
+
+
+
+Definition exit_rthread (st : state) (rid : rthreadptr) (vp : valptr) :=
+  update_rthread st rid {| rt_code := Val vp ; rt_cont := Kid |}.
+
+Definition addval (st : state) (v : value) :=
+  ({|
+      st_rthreads := st.(st_rthreads) ;
+      st_vals := st.(st_vals) ++ v :: nil ;
+      st_freename := st.(st_freename) ;
+    |}, length st.(st_vals)).
+
+Definition is_finished (st : state) (rid : rthreadptr) :=
+  match nth_error st.(st_rthreads) rid with
+  | None => None
+  | Some rthread =>
+    match rthread.(rt_code), rthread.(rt_cont) with
+    | Val vp, Kid => Some vp
+    | _, _ => None
+    end
+  end.
+
+Definition fst3 {A B C : Type} (x : A * B * C) := fst (fst x).
+Definition snd3 {A B C : Type} (x : A * B * C) := snd (fst x).
+Definition thd3 {A B C : Type} (x : A * B * C) := snd x.
+
+Definition step_r (st : state) (rid : rthreadptr) : state :=
+  match nth_error st.(st_rthreads) rid with
+  | None => st
+  | Some rthread =>
+    match rthread.(rt_code) with
+    | Term (app u v) e =>
+      let st2vp := makelazy st v e in
+      update_rthread (fst st2vp) rid {| rt_code := Term u e ; rt_cont := Kapp (snd st2vp) rthread.(rt_cont) |}
+    | Term (abs u) e =>
+      match rthread.(rt_cont) with
+      | Kswitch _ _ _ _ => st (* type error *)
+      | Kid =>
+        let st2yfv := freevar st in
+        let st3vp := makelazy (fst3 st2yfv) u ((thd3 st2yfv) :: e) in
+        let st4vp2 := addval (fst st3vp) (Clos u e (snd3 st2yfv) (snd st3vp)) in
+        exit_rthread (fst st4vp2) rid (snd st4vp2)
+      | Kapp v c =>
+        update_rthread st rid {| rt_code := Term u (v :: e) ; rt_cont := c |}
+      end
+    | Term (var n) e =>
+      match nth_error e n with
+      | None => st (* variable not found *)
+      | Some vp =>
+        update_rthread st rid {| rt_code := Val vp ; rt_cont := rthread.(rt_cont) |}
+      end
+    | Term (dvar n) e =>
+      st (* todo use defs *)
+    | Term _ e => st (* todo *)
+    | Val vp =>
+      match nth_error st.(st_vals) vp with
+      | None => st (* value not found *)
+      | Some (Thread rid2) =>
+        match is_finished st rid2 with
+        | None => st (* Thread is not finished yet, wait *)
+        | Some vp2 =>
+          update_rthread st rid {| rt_code := Val vp2 ; rt_cont := rthread.(rt_cont) |}
+        end
+      | Some (Clos u e y vp) =>
+        match rthread.(rt_cont) with
+        | Kid => st (* should be impossible? TODO *)
+        | Kswitch _ _ _ _  => st (* type error *)
+        | Kapp v c =>
+          update_rthread st rid {| rt_code := Term u (v :: e) ; rt_cont := c |}
+        end
+      | Some _ => st (* todo *)
+      end
+    end
+  end.
+
+Inductive step : state -> state -> Prop :=
+| step_rthread :
+    forall st rid, rid < length st.(st_rthreads) -> step st (step_r st rid).
+
+
+
+
+Inductive read_addr st : addr -> term -> Prop :=
+| read_thread_val : forall rid vp c t h,
+    nth_error st.(st_rthreads) rid = Some {| rt_code := Val vp ; rt_cont := c |} ->
+    read_addr st (a_val vp) t ->
+    read_cont st c h ->
+    read_addr st (a_rthread rid) (fill_hctx h t)
+| read_thread_term : forall rid e el c t h,
+    nth_error st.(st_rthreads) rid = Some {| rt_code := Term t e ; rt_cont := c |} ->
+    Forall2 (fun vp v => read_addr st (a_val vp) v) e el ->
+    read_cont st c h ->
+    read_addr st (a_rthread rid) (fill_hctx h (subst (read_env el) t))
+| read_val_thread :
+    forall vp rid t,
+      nth_error st.(st_vals) vp = Some (Thread rid) ->
+      read_addr st (a_rthread rid) t ->
+      read_addr st (a_val vp) t
+| read_val_clos :
+    forall vp t e el x vp2 t2,
+      nth_error st.(st_vals) vp = Some (Clos t e x vp2) ->
+      Forall2 (fun vp v => read_addr st (a_val vp) v) e el ->
+      read_addr st (a_val vp2) t2 ->
+      convertible beta (subst (read_env (dvar x :: el)) t) t2 ->
+      read_addr st (a_val vp) (subst (read_env el) (abs t))
+| read_val_neutral :
+    forall vp x c h uf,
+      nth_error st.(st_vals) vp = Some (Neutral {| n_id := x ; n_cont := c ; n_unfold := uf |}) ->
+      read_cont st c h ->
+      read_addr st (a_val vp) (fill_hctx h (dvar x))
+
+with read_cont st : cont -> hctx -> Prop :=
+| read_cont_kid : read_cont st Kid h_hole
+| read_cont_kapp :
+    forall vp c t h,
+      read_addr st (a_val vp) t ->
+      read_cont st c h ->
+      read_cont st (Kapp vp c) (compose_hctx h (h_app h_hole t))
+| read_cont_kswitch :
+    forall bs e bds c el h,
+      Forall2 (fun vp v => read_addr st (a_val vp) v) e el ->
+      read_cont st c h ->
+      read_cont st (Kswitch bs e bds c) (compose_hctx h (h_switch h_hole (map (fun '(p, t) => (p, subst (read_env el) t)) bs))).
+
+Lemma read_env_0 :
+  forall t e, read_env (t :: e) 0 = t.
+Proof.
+  intros; reflexivity.
+Qed.
+
+Lemma read_env_S :
+  forall t e n, read_env (t :: e) (S n) = read_env e n.
+Proof.
+  intros; reflexivity.
+Qed.
+
+Definition points st := points_to st.(st_rthreads) st.(st_vals).
+
+Definition no_delete st1 st2 :=
+  forall a, get_addr st2 a = None -> get_addr st1 a = None.
+
+Lemma no_delete_refl :
+  forall st, no_delete st st.
+Proof.
+  intros st a H; assumption.
+Qed.
+
+Lemma no_delete_iff :
+  forall st1 st2, no_delete st1 st2 <->
+             length st1.(st_rthreads) <= length st2.(st_rthreads) /\ length st1.(st_vals) <= length st2.(st_vals).
+Proof.
+  intros st1 st2. split.
+  - intros H. split.
+    + specialize (H (a_rthread (length (st_rthreads st2)))). simpl in H.
+      rewrite !nth_error_None in H. lia.
+    + specialize (H (a_val (length (st_vals st2)))). simpl in H.
+      rewrite !nth_error_None in H. lia.
+  - intros [H1 H2] [rid|vp] H; simpl in *; rewrite nth_error_None in *; lia.
+Qed.
+
+Lemma nth_error_app_Some :
+  forall (A : Type) (l1 l2 : list A) k x, nth_error l1 k = Some x -> nth_error (l1 ++ l2) k = Some x.
+Proof.
+  induction l1; intros l2 [|k] x; simpl in *; intros; try congruence.
+  apply IHl1; assumption.
+Qed.
+
+Lemma Forall2_impl_In_left_transparent :
+  forall (A B : Type) (P Q : A -> B -> Prop) L1 L2,
+    (forall x y, In x L1 -> P x y -> Q x y) -> Forall2 P L1 L2 -> Forall2 Q L1 L2.
+Proof.
+  intros A B P Q L1 L2 H Hforall. induction Hforall.
+  - constructor.
+  - econstructor.
+    + apply H; [left; reflexivity|assumption].
+    + apply IHHforall.
+      intros; eapply H; [right|]; eassumption.
+Defined.
+
+Lemma Forall2_In_left_transparent :
+  forall (A B : Type) (P : A -> B -> Prop) (Q : Prop) (L1 : list A) (L2 : list B) (x : A) (H : forall y, P x y -> Q), Forall2 P L1 L2 -> x ∈ L1 -> Q.
+Proof.
+  intros A B P Q L1 L2 x HQ H Hx; induction H.
+  - simpl in Hx; tauto.
+  - destruct Hx as [-> | Hx]; [eapply HQ; eassumption|apply (IHForall2 Hx)].
+Defined.
+
+Lemma read_cont_Acc :
+  forall st a c h, read_cont st c h -> cont_points_to c a -> (forall a t, read_addr st a t -> Acc (flip (points st)) a) -> Acc (flip (points st)) a.
+Proof.
+  intros st a c h Hread Hpoint Hrec. induction Hread; inversion Hpoint; subst.
+  - eapply Hrec; eassumption.
+  - apply IHHread. assumption.
+  - destruct a; simpl in *; [tauto|].
+    eapply Forall2_In_left_transparent; [|eassumption|eassumption].
+    intros; eapply Hrec, H0.
+  - tauto.
+Defined.
+
+Lemma read_addr_Acc :
+  forall st a t, read_addr st a t -> Acc (flip (points st)) a.
+Proof.
+  intros st. fix Hrec 3.
+  intros a t H; inversion H; subst; simpl; constructor; intros a2 Ha2; unfold flip in Ha2; simpl in Ha2; rewrite H0 in Ha2; inversion Ha2; subst; simpl in *.
+  - inversion H3; subst. eapply Hrec; eassumption.
+  - eapply read_cont_Acc; eassumption.
+  - inversion H3; subst.
+    destruct a2; simpl in *; [tauto|].
+    eapply Forall2_In_left_transparent; [|eassumption|eassumption].
+    intros; eapply Hrec, H4.
+  - eapply read_cont_Acc; eassumption.
+  - eapply Hrec; eassumption.
+  - destruct a2; simpl in *; [tauto|].
+    eapply Forall2_In_left_transparent; [|eassumption|eassumption].
+    intros; eapply Hrec, H4.
+  - eapply Hrec; eassumption.
+  - eapply read_cont_Acc; eassumption.
+Qed.
+
+Lemma read_cont_points_to :
+  forall st c h a, read_cont st c h -> cont_points_to c a -> exists t, read_addr st a t.
+Proof.
+  intros st c h a Hread Hpoint; induction Hread; simpl in *; inversion Hpoint; subst.
+  - eexists; eassumption.
+  - apply IHHread; assumption.
+  - destruct a; simpl in *; [tauto|].
+    eapply Forall2_In_left in H; [|eassumption].
+    destruct H; eexists; apply H.
+  - apply IHHread; assumption.
+Qed.
+
+Lemma read_addr_points_to :
+  forall st a1 t a2, read_addr st a1 t -> points st a1 a2 -> exists t2, read_addr st a2 t2.
+Proof.
+  intros st a1 t a2 Hread Hpoint; inversion Hread; subst; simpl in *; rewrite H in Hpoint.
+  - destruct Hpoint; simpl in *.
+    + inversion H2; subst. eexists; eassumption.
+    + eapply read_cont_points_to; eassumption.
+  - destruct Hpoint; simpl in *.
+    + inversion H2; subst.
+      destruct a2; simpl in *; [tauto|].
+      eapply Forall2_In_left in H0; [|eassumption].
+      destruct H0; eexists; apply H0.
+    + eapply read_cont_points_to; eassumption.
+  - inversion Hpoint; subst.
+    eexists; eassumption.
+  - inversion Hpoint; subst.
+    + destruct a2; simpl in *; [tauto|].
+      eapply Forall2_In_left in H0; [|eassumption].
+      destruct H0; eexists; apply H0.
+    + eexists; eassumption.
+  - inversion Hpoint; subst.
+    eapply read_cont_points_to; eassumption.
+Qed.
+
+Lemma read_addr_points_to_star :
+  forall st a1 t a2, read_addr st a1 t -> star (points st) a1 a2 -> exists t2, read_addr st a2 t2.
+Proof.
+  intros st a1 t a2 Hread H. revert t Hread; induction H; intros t Hread.
+  - eexists; eassumption.
+  - eapply read_addr_points_to in Hread; [|eassumption].
+    destruct Hread.
+    eapply IHstar; eassumption.
+Qed.
+
+Lemma Acc_cycle :
+  forall (A : Type) (R : A -> A -> Prop) x, plus R x x -> Acc (flip R) x -> False.
+Proof.
+  intros A R x Hplus Hacc. induction Hacc.
+  inversion Hplus; subst.
+  - eapply H0; eassumption.
+  - eapply H0; [eassumption|].
+    eapply plus_compose_star_right; [eassumption|].
+    apply star_1; assumption.
+Qed.
+
+Lemma update_case :
+  forall {A : Type} (l : list A) k1 k2 x, (k1 = k2 /\ nth_error (update l k1 x) k2 = Some x) \/ (nth_error (update l k1 x) k2 = nth_error l k2).
+Proof.
+  intros A l k1 k2 x.
+  destruct (Nat.eq_dec k1 k2).
+  + subst. rewrite nth_error_update2.
+    destruct nth_error; tauto.
+  + rewrite nth_error_update3 by assumption. tauto.
+Qed.
+
+
+
+Definition every_reachable st a (P : addr -> Prop) :=
+  forall a2, star (points st) a a2 -> P a2.
+Definition every_reachable_plus st a (P : addr -> Prop) :=
+  forall a2, plus (points st) a a2 -> P a2.
+
+Lemma every_reachable_impl :
+  forall st a (P Q : addr -> Prop),
+    (forall a2, star (points st) a a2 -> P a2 -> Q a2) -> every_reachable st a P -> every_reachable st a Q.
+Proof.
+  intros st a P Q H1 H2 a2 Hstar; apply H1; [assumption|]; apply H2; assumption.
+Qed.
+
+Lemma every_reachable_plus_impl :
+  forall st a (P Q : addr -> Prop),
+    (forall a2, plus (points st) a a2 -> P a2 -> Q a2) -> every_reachable_plus st a P -> every_reachable_plus st a Q.
+Proof.
+  intros st a P Q H1 H2 a2 Hplus; apply H1; [assumption|]; apply H2; assumption.
+Qed.
+
+Lemma every_reachable_star :
+  forall st a a2 P, star (points st) a a2 -> every_reachable st a P -> every_reachable st a2 P.
+Proof.
+  intros st a a2 P Hstar H a3 Hstar2. apply H. eapply star_compose; eassumption.
+Qed.
+
+Lemma every_reachable_plus_star :
+  forall st a a2 P, star (points st) a a2 -> every_reachable_plus st a P -> every_reachable_plus st a2 P.
+Proof.
+  intros st a a2 P Hstar H a3 Hplus. apply H. eapply plus_compose_star_left; eassumption.
+Qed.
+
+Lemma every_reachable_star_plus :
+  forall st a a2 P, plus (points st) a a2 -> every_reachable_plus st a P -> every_reachable st a2 P.
+Proof.
+  intros st a a2 P Hplus H a3 Hstar. apply H. eapply plus_compose_star_right; eassumption.
+Qed.
+
+Lemma every_reachable_plus_iff :
+  forall st a P, every_reachable_plus st a P <-> (forall a2, points st a a2 -> every_reachable st a2 P).
+Proof.
+  intros st a P. split; intros H.
+  - intros a2 Ha2 a3 Ha3. apply H. rewrite plus_star_iff. exists a2. split; assumption.
+  - intros a3 Ha3. rewrite plus_star_iff in Ha3; destruct Ha3 as (a2 & Ha2 & Ha3).
+    apply (H a2 Ha2 a3 Ha3).
+Qed.
+
+Lemma every_reachable_same :
+  forall st a P, every_reachable st a P -> P a.
+Proof.
+  intros st a P H; apply H, star_refl.
+Qed.
+
+Lemma every_reachable_is_plus :
+  forall st a P, every_reachable st a P -> every_reachable_plus st a P.
+Proof.
+  intros st a P H a2 Ha2. apply H, plus_star, Ha2.
+Qed.
+
+Lemma every_reachable_iff :
+  forall st a1 P, every_reachable st a1 P <-> P a1 /\ every_reachable_plus st a1 P.
+Proof.
+  intros st a1 P. split; intros H.
+  - split; [eapply every_reachable_same|eapply every_reachable_is_plus]; eassumption.
+  - intros a2 Ha2. inversion Ha2; subst; [tauto|].
+    apply H. rewrite plus_star_iff; eexists; split; eassumption.
+Qed.
+
+
+Definition unchanged_from st1 st2 a := every_reachable st1 a (fun a2 => get_addr st1 a2 = get_addr st2 a2).
+Definition unchanged_from_plus st1 st2 a := every_reachable_plus st1 a (fun a2 => get_addr st1 a2 = get_addr st2 a2).
+
+Lemma unchanged_from_same :
+  forall st1 st2 a, unchanged_from st1 st2 a -> get_addr st1 a = get_addr st2 a.
+Proof.
+  intros st1 st2 a. apply every_reachable_same.
+Qed.
+
+Lemma unchanged_from_points :
+  forall st1 st2 a1 a2, unchanged_from st1 st2 a1 -> points st1 a1 a2 -> unchanged_from st1 st2 a2.
+Proof.
+  intros st1 st2 a1 a2 Hchanged Hpoint.
+  apply every_reachable_is_plus in Hchanged.
+  eapply every_reachable_plus_iff in Hchanged; eassumption.
+Qed.
+
+Definition unchanged_read st1 st2 a := every_reachable st1 a (fun a2 => forall t, read_addr st1 a t -> read_addr st2 a t).
+Definition unchanged_read_plus st1 st2 a := every_reachable_plus st1 a (fun a2 => forall t, read_addr st1 a t -> read_addr st2 a t).
+
+Lemma read_cont_same :
+  forall st1 st2 c h,
+    read_cont st1 c h ->
+    (forall a t, read_addr st1 a t -> cont_points_to c a -> read_addr st2 a t) ->
+    read_cont st2 c h.
+Proof.
+  intros st1 st2 c h Hread H; induction Hread.
+  - constructor.
+  - econstructor.
+    + apply H; [assumption|]. apply kapp_points_to_1.
+    + apply IHHread. intros; apply H, kapp_points_to_2; assumption.
+  - econstructor.
+    + eapply Forall2_impl_In_left_transparent; [|eassumption].
+      intros; apply H; [assumption|]. apply kswitch_points_to_1. assumption.
+    + apply IHHread. intros; apply H, kswitch_points_to_2; assumption.
+Defined.
+
+Lemma read_addr_same :
+  forall st1 st2 a t, read_addr st1 a t -> unchanged_from st1 st2 a -> read_addr st2 a t.
+Proof.
+  intros st1 st2 a t H Hchanged.
+  assert (Hacc := read_addr_Acc _ _ _ H).
+  revert t H. induction Hacc; intros t Hread.
+  assert (Hrec : forall y, points st1 x y -> forall t, read_addr st1 y t -> read_addr st2 y t).
+  { intros; apply H0; [|eapply unchanged_from_points|]; eassumption. }
+  inversion Hread; subst.
+  - eapply read_thread_val.
+    + rewrite (unchanged_from_same _ _ _ Hchanged) in H1. eassumption.
+    + apply Hrec; [|assumption].
+      simpl; rewrite H1. left; constructor.
+    + eapply read_cont_same; [eassumption|].
+      intros; apply Hrec; [|assumption].
+      simpl; rewrite H1. right; assumption.
+  - eapply read_thread_term.
+    + rewrite (unchanged_from_same _ _ _ Hchanged) in H1. eassumption.
+    + eapply Forall2_impl_In_left_transparent; [|eassumption].
+      intros vp t Hvp; apply Hrec.
+      simpl; rewrite H1. left; constructor; assumption.
+    + eapply read_cont_same; [eassumption|].
+      intros; apply Hrec; [|assumption].
+      simpl; rewrite H1. right; assumption.
+  - eapply read_val_thread.
+    + rewrite (unchanged_from_same _ _ _ Hchanged) in H1. eassumption.
+    + apply Hrec; [|assumption].
+      simpl; rewrite H1. constructor.
+  - eapply read_val_clos.
+    + rewrite (unchanged_from_same _ _ _ Hchanged) in H1. eassumption.
+    + eapply Forall2_impl_In_left_transparent; [|eassumption].
+      intros; apply Hrec; [|assumption].
+      simpl; rewrite H1. constructor; assumption.
+    + eapply Hrec; [|eassumption].
+      simpl; rewrite H1. apply clos_points_to_2.
+    + assumption.
+  - eapply read_val_neutral.
+    + rewrite (unchanged_from_same _ _ _ Hchanged) in H1. eassumption.
+    + eapply read_cont_same; [eassumption|].
+      intros; apply Hrec; [|assumption].
+      simpl; rewrite H1. constructor; assumption.
+Qed.
+
+Definition unchanged_from_plus st1 st2 a :=
+  forall a2, points_to st1.(st_rthreads) st1.(st_vals) a a2 -> unchanged_from st1 st2 a2.
+
+Lemma read_addr_same_Forall2 :
+  forall st1 st2 e el,
+    Forall2 (fun vp t => read_addr st1 (a_val vp) t) e el ->
+    (forall vp, In vp e -> unchanged_from st1 st2 (a_val vp)) ->
+    Forall2 (fun vp t => read_addr st2 (a_val vp) t) e el.
+Proof.
+  intros st1 st2 e el Hall Hchange.
+  eapply Forall2_impl_In_left_transparent; [|eassumption].
+  intros; eapply read_addr_same; [apply H0|apply Hchange; assumption].
+Qed.
+
+Lemma unchanged_from_trans :
+  forall st1 st2 st3 a, unchanged_from st1 st2 a -> unchanged_from st2 st3 a -> unchanged_from st1 st3 a.
+Proof.
+  intros st1 st2 st3 a H1 H2 [rid|vp] Ha2; simpl.
+  - etransitivity; [eapply (H1 (a_rthread _)); eassumption|eapply (H2 (a_rthread _))].
+    clear H2.
+    induction Ha2.
+    + apply star_refl.
+    + econstructor; [|eapply IHHa2; eapply unchanged_from_points_to; eassumption].
+      destruct x; simpl in *; rewrite (unchanged_from_same _ _ _ H1) in H; assumption.
+  - etransitivity; [eapply (H1 (a_val _)); eassumption|eapply (H2 (a_val _))].
+    clear H2.
+    induction Ha2.
+    + apply star_refl.
+    + econstructor; [|eapply IHHa2; eapply unchanged_from_points_to; eassumption].
+      destruct x; simpl in *; rewrite (unchanged_from_same _ _ _ H1) in H; assumption.
+Qed.
+
+Lemma unchanged_from_cycle :
+  forall st a1 v a2 t, plus (points_to st.(st_rthreads) st.(st_vals)) a1 a2 -> read_addr st a1 t -> unchanged_from st (update_addr st a1 v) a2.
+Proof.
+  intros st a1 v a2 t Hplus Hread a3 Ha3.
+  destruct a1 as [rid|vp]; destruct a3 as [rid2|vp2]; simpl in *; try reflexivity.
+  - destruct (update_case st.(st_rthreads) rid rid2 v).
+    + destruct H; subst. exfalso.
+      eapply Acc_cycle; [eapply plus_compose_star_right; eassumption|].
+      eapply read_addr_Acc; eassumption.
+    + congruence.
+  - destruct (update_case st.(st_vals) vp vp2 v).
+    + destruct H; subst. exfalso.
+      eapply Acc_cycle; [eapply plus_compose_star_right; eassumption|].
+      eapply read_addr_Acc; eassumption.
+    + congruence.
+Qed.
+
+Lemma unchanged_from_plus_cycle :
+  forall st a1 v a2 t, star (points_to st.(st_rthreads) st.(st_vals)) a1 a2 -> read_addr st a1 t -> unchanged_from_plus st (update_addr st a1 v) a2.
+Proof.
+  intros st a1 v a2 t Hstar Hread a3 Hpoint.
+  eapply unchanged_from_cycle; [|eassumption].
+  eapply plus_compose_star_left; [eassumption|].
+  apply plus_1; assumption.
+Qed.
+
+Lemma unchanged_from_plus_update :
+  forall st a v t, read_addr st a t -> unchanged_from_plus st (update_addr st a v) a.
+Proof.
+  intros; eapply unchanged_from_plus_cycle; [|eassumption].
+  apply star_refl.
+Qed.
+
+Lemma unchanged_from_plus_trans :
+  forall st1 st2 st3 a, unchanged_from st1 st2 a -> unchanged_from_plus st2 st3 a -> unchanged_from_plus st1 st3 a.
+Proof.
+  intros st1 st2 st3 a H12 H23 a2 Ha2.
+  eapply unchanged_from_trans; [eapply unchanged_from_points_to; eassumption|apply H23].
+  destruct a; simpl in *; rewrite (unchanged_from_same _ _ _ H12) in Ha2; assumption.
+Qed.
+
+Lemma nth_error_extend :
+  forall {A : Type} (l : list A) x, nth_error (l ++ x :: nil) (length l) = Some x.
+Proof.
+  intros A l x. rewrite nth_error_app2 by lia.
+  destruct (length l - length l) eqn:Hll; [reflexivity|lia].
+Qed.
+
+Lemma unchanged_from_addval :
+  forall st v a t, read_addr st a t -> unchanged_from st (fst (addval st v)) a.
+Proof.
+  intros st v a t Hread a2 Ha2.
+  eapply read_addr_points_to_star in Ha2; [|eassumption].
+  destruct Ha2 as (t2 & Ha2).
+  destruct a2 as [rid|vp]; [reflexivity|].
+  simpl.
+  inversion Ha2; subst; erewrite nth_error_app_Some; eassumption.
+Qed.
+
+Lemma unchanged_from_makelazy :
+  forall st t e a t2,
+    read_addr st a t2 ->
+    unchanged_from st (fst (makelazy st t e)) a.
+Proof.
+  intros st t e a t2 Hread a2 Ha2.
+  eapply read_addr_points_to_star in Ha2; [|eassumption].
+  destruct Ha2 as (t3 & Ha2).
+  inversion Ha2; simpl; subst; erewrite nth_error_app_Some; eassumption.
+Qed.
+
+Definition stable_partial st1 st2 st3 a :=
+  no_delete st1 st2 /\ no_delete st2 st3 /\
+  forall a2,
+    (get_addr st2 a2 = get_addr st1 a2 \/
+     ((get_addr st1 a2 = None \/ star (points st1) a a2) /\
+      forall a3, points st2 a2 a3 -> star (points st1) a a3 \/ get_addr st1 a3 = None)) /\
+    (get_addr st3 a2 = get_addr st2 a2 \/
+     ((get_addr st1 a2 = None \/ star (points st1) a a2) /\
+      forall a3, points st3 a2 a3 -> star (points st1) a a3 \/ get_addr st1 a3 = None)).
+
+Definition stable st1 st2 a := stable_partial st1 st1 st2 a.
+
+(*
+Definition stable st1 st2 a :=
+  no_delete st1 st2 /\
+  forall a2,
+    (get_addr st2 a2 = get_addr st1 a2 \/
+     ((get_addr st1 a2 = None \/ star (points_to st1.(st_rthreads) st1.(st_vals)) a a2) /\
+      forall a3, points st2 a2 a3 ->
+            get_addr st1 a3 = None \/ star (points_to st1.(st_rthreads) st1.(st_vals)) a a3)).
+ *)
+
+(*
+Lemma stable_partial_refl :
+  forall st1 st2 a, no_delete st1 st2 -> stable_partial st1 st2 st2 a.
+Proof.
+  intros st1 st2 a Hdel.
+  split; [apply Hdel|].
+  split; [apply no_delete_refl|].
+  intros a2. split; [|left; reflexivity].
+  left; reflexivity.
+Qed.
+ *)
+
+Lemma stable_refl :
+  forall st a, stable st st a.
+Proof.
+  intros.
+  split; [apply no_delete_refl|].
+  split; [apply no_delete_refl|].
+  intros a2. split; left; reflexivity.
+Qed.
+
+
+Definition a_points_to (a : addr) (v : match a return Type with a_rthread _ => rthread | a_val _ => value end) :=
+  match a, v with a_rthread _, v => rthread_points_to v | a_val _, v => val_points_to v end.
+
+Lemma get_addr_points :
+  forall st1 st2 a1 a2, get_addr st1 a1 = get_addr st2 a1 -> points st1 a1 a2 <-> points st2 a1 a2.
+Proof.
+  intros st1 st2 [rid|vp] a2 H; simpl in *; rewrite H; reflexivity.
+Qed.
+
+Lemma get_addr_points2 :
+  forall st a1 a2, points st a1 a2 <-> match get_addr st a1 with None => False | Some v => a_points_to a1 v a2 end.
+Proof.
+  intros st [rid|vp] a2; simpl; reflexivity.
+Qed.
+
+
+Lemma stable_partial_path :
+  forall st1 st2 st3 a1 a2,
+    stable_partial st1 st2 st3 a1 ->
+    star (points st3) a1 a2 ->
+    star (points st1) a1 a2 \/ get_addr st1 a2 = None.
+Proof.
+  intros st1 st2 st3 a1 a2 (Hdel1 & Hdel2 & Hstable) Hstar.
+  apply star_flip in Hstar. induction Hstar.
+  - left. apply star_refl.
+  - specialize (IHHstar Hstable).
+    destruct (Hstable y) as [[Hy1 | [Hy1a Hy1b]] [Hy2 | [Hy2a Hy2b]]].
+    + eapply get_addr_points in H; [|symmetry; eassumption].
+      destruct IHHstar;
+        [|eapply get_addr_points in H; [|symmetry; eassumption]; destruct y; simpl in *; rewrite H0 in H; tauto].
+      left. eapply star_compose; [eassumption|apply star_1].
+      eapply get_addr_points; [symmetry|]; eassumption.
+    + apply Hy2b. assumption.
+    + apply Hy1b. eapply get_addr_points; [symmetry|]; eassumption.
+    + apply Hy2b. assumption.
+Qed.
+
+(*
+Lemma stable_path :
+  forall st1 st2 a1 a2,
+    stable st1 st2 a1 ->
+    star (points_to st2.(st_rthreads) st2.(st_vals)) a1 a2 ->
+    get_addr st1 a2 = None \/ star (points_to st1.(st_rthreads) st1.(st_vals)) a1 a2.
+Proof.
+  intros st1 st2 a1 a2 Hstable Hstar.
+  apply star_flip in Hstar. induction Hstar.
+  - right. apply star_refl.
+  - specialize (IHHstar Hstable).
+    destruct (Hstable y) as [HyNone [Hy | [Hy1 Hy2]]].
+    + right. eapply get_addr_points_to in H; [|symmetry; eassumption].
+      destruct IHHstar; [|eapply star_compose; [eassumption|apply star_1; eassumption]].
+      destruct y; simpl in *; rewrite H0 in H; tauto.
+    + apply Hy2. assumption.
+Qed.
+ *)
+(*
+Lemma stable_path_ext :
+  forall st1 st2 a1 a2,
+    stable st1 st2 a1 ->
+    get_addr st2 a2 = None \/ star (points_to st2.(st_rthreads) st2.(st_vals)) a1 a2 ->
+    get_addr st1 a2 = None \/ star (points_to st1.(st_rthreads) st1.(st_vals)) a1 a2.
+Proof.
+  intros st1 st2 a1 a2 Hstable [H | H].
+  - left. apply Hstable. assumption.
+  - eapply stable_path; eassumption.
+Qed.
+ *)
+
+Lemma stable_partial_path_ext :
+  forall st1 st2 st3 a1 a2,
+    stable_partial st1 st2 st3 a1 ->
+    star (points st3) a1 a2 \/ get_addr st3 a2 = None ->
+    star (points st1) a1 a2 \/ get_addr st1 a2 = None.
+Proof.
+  intros st1 st2 st3 a1 a2 Hstable [H | H].
+  - eapply stable_partial_path in H; eassumption.
+  - right; apply Hstable, Hstable; assumption.
+Qed.
+
+Definition stable_partial_weak st1 st2 st3 a :=
+  no_delete st2 st3 /\
+  forall a2,
+    (get_addr st3 a2 = get_addr st2 a2 \/
+     ((get_addr st1 a2 = None \/ star (points st1) a a2) /\
+      forall a3, points st3 a2 a3 -> star (points st1) a a3 \/ get_addr st1 a3 = None)).
+
+Lemma stable_partial_trans :
+  forall st1 st2 st3 st4 a, stable_partial st1 st2 st3 a -> stable_partial_weak st1 st3 st4 a -> stable_partial st1 st2 st4 a.
+Proof.
+  intros st1 st2 st3 st4 a (H1a & H1b & H1c) (H2a & H2b).
+  split; [apply H1a|].
+  split; [intros a2 Ha2; apply H1b, H2a; assumption|].
+  intros a2. split; [apply H1c|].
+  destruct (H2b a2) as [H2b1 | H2b2].
+  - destruct (H1c a2) as [H1c1 [H1c2a | [H1c2b1 H1c2b2]]].
+    + left. congruence.
+    + right. split; [assumption|].
+      intros a3 Ha3; apply H1c2b2.
+      eapply get_addr_points; [symmetry|]; eassumption.
+  - right. assumption.
+Qed.
+
+Lemma stable_partial_trans_flipped :
+  forall st1 st2 st3 st4 a, stable_partial_weak st1 st3 st4 a -> stable_partial st1 st2 st3 a -> stable_partial st1 st2 st4 a.
+Proof.
+  intros; eapply stable_partial_trans; eassumption.
+Qed.
+
+
+(*
+Lemma stable_trans :
+  forall st1 st2 st3 a, stable st1 st2 a -> stable st2 st3 a -> stable st1 st3 a.
+Proof.
+  intros st1 st2 st3 a H1 H2 a2.
+  split; [intros; apply H1, H2; assumption|].
+  destruct (H2 a2) as [Ha2Noneb [Ha2b | [Ha2b1 Ha2b2]]].
+  - destruct (H1 a2) as [Ha2Nonea [Ha2a | [Ha2a1 Ha2a2]]].
+    + left. congruence.
+    + right. split; [assumption|].
+      intros a3 Ha3; apply Ha2a2.
+      eapply get_addr_points_to; [|eassumption].
+      symmetry; assumption.
+  - destruct (H1 a2) as [Ha2Nonea [Ha2a | [Ha2a1 Ha2a2]]].
+    + right. eapply stable_path_ext in Ha2b1; [|eassumption].
+      split; [assumption|].
+      intros; eapply stable_path_ext; [eassumption|apply Ha2b2; assumption].
+    + right. split; [assumption|].
+      intros a3 Ha3. eapply Ha2b2, stable_path_ext in Ha3; eassumption.
+Qed.
+ *)
+
+Lemma stable_partial_stable :
+  forall st1 st2 st3 a, stable_partial st1 st2 st3 a -> stable st1 st3 a.
+Proof.
+  intros st1 st2 st3 a (H1 & H2 & H3).
+  split; [apply no_delete_refl|].
+  split; [intros a2 Ha2; apply H1, H2; assumption|].
+  intros a2.
+  split; [left; reflexivity|].
+  destruct (H3 a2) as [H3a [H3b1 | [H3b2a H3b2b]]].
+  - destruct H3a as [H3a1 | [H3a2a H3a2b]].
+    + left; congruence.
+    + right. split; [assumption|].
+      intros a3 Ha3; apply H3a2b.
+      eapply get_addr_points; [symmetry|]; eassumption.
+  - right. split; assumption.
+Qed.
+
+Lemma stable_partial_stable_trans :
+  forall st1 st2 st3 st4 a,
+    stable_partial st1 st2 st3 a -> stable st3 st4 a -> stable_partial st1 st2 st4 a.
+Proof.
+  intros st1 st2 st3 st4 a H123 H34.
+  inversion H123 as (H1 & H2 & H3).
+  inversion H34 as (H4 & H5 & H6).
+  eapply stable_partial_trans; [split; [|split]; eassumption|].
+  split; [assumption|].
+  intros a2. destruct (H6 a2) as [H6a [H6b1 | [H6b2a H6b2b]]].
+  - left; assumption.
+  - right. eapply or_comm, stable_partial_path_ext, or_comm in H6b2a; [|eassumption].
+    split; [assumption|].
+    intros a3 Ha3. eapply stable_partial_path_ext; [eassumption|].
+    apply H6b2b; assumption.
+Qed.
+
+(*
+Lemma stable_stable_partial :
+  forall st1 st2 st3 a, no_delete st3 st1 -> stable st1 st2 a -> stable_partial st3 st1 st2 a.
+Proof.
+  intros st1 st2 st3 a H (_ & H1 & H2).
+  split; [apply H|].
+  split; [apply H1|].
+  intros a2.
+  destruct (H2 a2) as [Ha2 | [Ha2a Ha2b]].
+  - left. assumption.
+  - right. split.
+    + destruct Ha2a as [Ha2a | Ha2a]; [left; apply H; assumption|].
+    destruct Ha2a.
+    + 
+    split; [|assumption].
+    destruct Ha2a; [|right; assumption].
+    left; apply H; assumption.
+Qed.
+ *)
+
+(*
+Lemma stable_trans :
+  forall st1 st2 st3 a, no_delete st1 st2 -> stable st1 st2 a -> stable st2 st3 a -> stable st1 st3 a.
+Proof.
+  intros. eapply stable_partial_trans; [eassumption|].
+  apply stable_stable_partial; assumption.
+Qed.
+ *)
+
+Lemma get_update_addr_eq :
+  forall st a v1 v2, get_addr st a = Some v1 -> get_addr (update_addr st a v2) a = Some v2.
+Proof.
+  intros. destruct a; eapply nth_error_update; eassumption.
+Qed.
+
+Lemma get_update_addr_eq2 :
+  forall st a v, get_addr (update_addr st a v) a = match get_addr st a with None => None | Some _ => Some v end.
+Proof.
+  intros. destruct a; eapply nth_error_update2; eassumption.
+Qed.
+
+Lemma get_update_addr_eq3 :
+  forall st a1 a2 v, a1 <> a2 -> get_addr (update_addr st a2 v) a1 = get_addr st a1.
+Proof.
+  intros. destruct a1, a2; simpl in *; try reflexivity; eapply nth_error_update3; congruence.
+Qed.
+
+Lemma addr_eq_dec :
+  forall (a1 a2 : addr), { a1 = a2 } + { a1 <> a2 }.
+Proof.
+  intros [x|x] [y|y]; try (right; congruence);
+    destruct (Nat.eq_dec x y); constructor; congruence.
+Qed.
+
+Lemma stable_update :
+  forall st1 st2 a1 a2 v,
+    get_addr st1 a2 = None \/ star (points st1) a1 a2 ->
+    (forall a3, a_points_to a2 v a3 -> star (points st1) a1 a3 \/ get_addr st1 a3 = None) ->
+    stable_partial_weak st1 st2 (update_addr st2 a2 v) a1.
+Proof.
+  intros st1 st2 a1 a2 v H1 H2.
+  split.
+  - intros a3 Ha3; destruct (addr_eq_dec a3 a2).
+    + subst. rewrite get_update_addr_eq2 in Ha3. destruct (get_addr st2 a2); congruence.
+    + rewrite get_update_addr_eq3 in Ha3; assumption.
+  - intros a3. destruct (addr_eq_dec a3 a2).
+    + subst. right. split; [assumption|].
+      intros a3 Ha3.
+      rewrite get_addr_points2, get_update_addr_eq2 in Ha3.
+        destruct (get_addr st2 a2); [|tauto].
+        apply H2; assumption.
+    + left. rewrite get_update_addr_eq3; [reflexivity|assumption].
+Qed.
+
+Lemma nth_error_extend_case :
+  forall {A : Type} l (x : A) n,
+    nth_error (l ++ x :: nil) n = nth_error l n \/ (n = length l /\ nth_error (l ++ x :: nil) n = Some x).
+Proof.
+  intros A l x n.
+  destruct (le_lt_dec (length l) n).
+  - rewrite nth_error_app2 by assumption.
+    destruct (n - length l) eqn:Hn; simpl; [right; split; [lia|reflexivity]|].
+    left. destruct n0; symmetry; apply nth_error_None; assumption.
+  - left. rewrite nth_error_app1; tauto.
+Qed.
+
+Lemma stable_addval :
+  forall st1 st2 a v,
+    length (st1.(st_vals)) <= length (st2.(st_vals)) ->
+    (forall a2, val_points_to v a2 -> star (points st1) a a2 \/ get_addr st1 a2 = None) ->
+    stable_partial_weak st1 st2 (fst (addval st2 v)) a.
+Proof.
+  intros st1 st2 a v Hlen H.
+  split.
+  - intros a2 Ha2.
+    destruct a2; simpl in *; [assumption|].
+    rewrite nth_error_None in *. rewrite app_length in Ha2. lia.
+  - intros a2. destruct a2 as [rid|vp]; simpl in *; [left; reflexivity|].
+    destruct (nth_error_extend_case (st_vals st2) v vp) as [-> | [-> ->]].
+    + left. reflexivity.
+    + right. split; [|assumption].
+      left. rewrite nth_error_None. lia.
+Qed.
+
+Lemma stable_makelazy :
+  forall st1 st2 a t e,
+    length (st1.(st_rthreads)) <= length (st2.(st_rthreads)) ->
+    length (st1.(st_vals)) <= length (st2.(st_vals)) ->
+    (forall a2, env_points_to e a2 -> star (points st1) a a2 \/ get_addr st1 a2 = None) ->
+    stable_partial_weak st1 st2 (fst (makelazy st2 t e)) a.
+Proof.
+  intros st1 st2 a t e Hlen1 Hlen2 H.
+  split.
+  - intros a2 Ha2.
+    destruct a2; simpl in *; rewrite nth_error_None in *; rewrite app_length in Ha2; lia.
+  - intros [rid|vp]; simpl in *.
+    + destruct (nth_error_extend_case (st_rthreads st2) {| rt_code := Term t e; rt_cont := Kid |} rid) as [-> | [-> ->]].
+      * left. reflexivity.
+      * right. split; [left; rewrite nth_error_None; lia|].
+        intros a2 [Ha2 | Ha2]; inversion Ha2; subst.
+        apply H. assumption.
+    + destruct (nth_error_extend_case (st_vals st2) (Thread (length (st_rthreads st2))) vp) as [-> | [-> ->]].
+      * left. reflexivity.
+      * right. split; [left; rewrite nth_error_None; lia|].
+        intros a2 Ha2; inversion Ha2; subst.
+        right. simpl. rewrite nth_error_None. lia.
+Qed.
+
+
+Lemma step_r_stable :
+  forall st rid, stable st (step_r st rid) (a_rthread rid).
+Proof.
+  intros st rid. unfold step_r.
+  destruct nth_error as [[code cont]|] eqn:Hrid; [|apply stable_refl].
+  destruct code as [t e|vp].
+  - destruct t; cbv beta delta [rt_code rt_cont] iota.
+    + destruct (nth_error e n) as [vp|] eqn:He; [|apply stable_refl].
+      eapply stable_partial_trans; [apply stable_refl|].
+      apply stable_update; [right; apply star_refl|].
+      intros a3 [Ha3 | Ha3].
+      * inversion Ha3; subst. left. apply star_1.
+        simpl. rewrite Hrid. left. constructor.
+        eapply nth_error_In; eassumption.
+      * left. apply star_1. simpl. rewrite Hrid. right. assumption.
+    + apply stable_refl.
+    + destruct cont.
+      * eapply stable_partial_trans_flipped.
+        {
+          apply stable_update; [right; apply star_refl|].
+          intros a3 [Ha3 | Ha3]; inversion Ha3; subst.
+          simpl. rewrite nth_error_None, !app_length; lia.
+        }
+        eapply stable_partial_trans_flipped.
+        {
+          apply stable_addval; [simpl; rewrite !app_length; lia|].
+          intros a2 Ha2. inversion Ha2; subst.
+          -- left. apply star_1. simpl. rewrite Hrid. left. constructor. assumption.
+          -- right. simpl. rewrite nth_error_None, app_length. lia.
+        }
+        eapply stable_partial_trans_flipped.
+        {
+          apply stable_makelazy; [simpl; lia|simpl; rewrite app_length; lia|].
+          intros [rid2|vp2]; [intros [] | intros [H | H]]; simpl in *.
+          -- subst. right. rewrite nth_error_None; lia.
+          -- left. apply star_1. simpl. rewrite Hrid. left. constructor. assumption.
+        }
+        eapply stable_partial_trans_flipped; [|apply stable_refl].
+        apply stable_addval; [lia|].
+        intros a2 Ha2; inversion Ha2; subst. inversion H0.
+      * eapply stable_partial_trans_flipped; [|apply stable_refl].
+        apply stable_update; [right; apply star_refl|].
+        intros a3 [Ha3 | Ha3]; left; apply star_1.
+        -- inversion Ha3; subst.
+           destruct a3; simpl in *; [tauto|]. rewrite Hrid.
+           destruct H2 as [H2 | H2]; [subst; right; constructor|].
+           left. constructor. assumption.
+        -- simpl. rewrite Hrid. right. constructor. assumption.
+      * apply stable_refl.
+    + eapply stable_partial_trans_flipped.
+      {
+        apply stable_update; [right; apply star_refl|].
+        intros a3 [Ha3 | Ha3].
+        * inversion Ha3; subst. left. apply star_1. simpl. rewrite Hrid. left. constructor. assumption.
+        * inversion Ha3; subst; [right; simpl; rewrite nth_error_None; lia|].
+          left. apply star_1. simpl. rewrite Hrid. right. assumption.
+      }
+      eapply stable_partial_trans_flipped; [|apply stable_refl].
+      apply stable_makelazy; [lia|lia|].
+      intros a3 Ha3; left; apply star_1. simpl. rewrite Hrid. left. constructor. assumption.
+    + admit.
+    + admit.
+  - cbv beta delta [rt_code rt_cont] iota.
+    destruct (nth_error st.(st_vals) vp) as [v|] eqn:Hvp; [|apply stable_refl].
+    destruct v.
+    + destruct is_finished as [v|] eqn:Hfinished; [|apply stable_refl].
+      eapply stable_partial_trans_flipped; [|apply stable_refl].
+      apply stable_update; [right; apply star_refl|].
+      intros a3 [Ha3 | Ha3]; [|left; apply star_1; simpl; rewrite Hrid; right; assumption].
+      inversion Ha3; subst. unfold is_finished in Hfinished.
+      destruct (nth_error (st_rthreads st) r) as [[code1 cont1]|]eqn:Hr; [|congruence].
+      simpl in Hfinished.
+      destruct code1 as [? ?|vp2]; [congruence|].
+      destruct cont1; try congruence. injection Hfinished as Hfinished. subst.
+      left.
+      econstructor; [simpl; rewrite Hrid; left; constructor|].
+      econstructor; [simpl; rewrite Hvp; constructor|].
+      apply star_1. simpl. rewrite Hr. left. constructor.
+    + admit.
+    + destruct cont.
+      * admit.
+      * eapply stable_partial_trans_flipped; [|apply stable_refl].
+        apply stable_update; [right; apply star_refl|].
+        intros a3 [Ha3 | Ha3]; [|left; apply star_1; simpl; rewrite Hrid; right; constructor; assumption].
+        inversion Ha3; subst. destruct a3; simpl in *; [tauto|].
+        destruct H2 as [H2 | H2]; [left; apply star_1; simpl; rewrite Hrid; subst; right; constructor|].
+        left. econstructor; simpl; [rewrite Hrid; left; constructor|].
+        apply star_1. simpl. rewrite Hvp. apply clos_points_to_1. assumption.
+      * apply stable_refl.
+    + admit.
+Admitted.
+
+
+
+Lemma and_left :
+  forall (A B : Prop), A -> (A -> B) -> A /\ B.
+Proof.
+  intros A B HA HB; split; [apply HA|apply HB, HA].
+Qed.
+
+Lemma and_right :
+  forall (A B : Prop), (B -> A) -> B -> A /\ B.
+Proof.
+  intros A B HA HB; split; [apply HA, HB|apply HB].
+Qed.
+
+Ltac and_left := apply and_left.
+Ltac and_right := apply and_right.
+Tactic Notation "and_left" "as" simple_intropattern(p) := and_left; [|intros p].
+Tactic Notation "and_right" "as" simple_intropattern(p) := and_right; [intros p|].
+
+
+
+Lemma step_r_beta_hnf :
+  forall st st2 rid t,
+    step_r st rid = st2 ->
+    read_addr st (a_rthread rid) t ->
+    every_reachable_plus st (a_rthread rid) (fun a => forall t, read_addr st a t -> read_addr st2 a t) /\
+    exists t2, read_addr st2 (a_rthread rid) t2 /\ reflc beta_hnf t t2.
+Proof.
+  intros st st2 rid t <- Hread.
+  match goal with [ |- ?G ] => assert (Hsame : every_reachable st (a_rthread rid) (fun a => forall t, read_addr st a t -> read_addr (step_r st rid) a t) -> G) end.
+  {
+    intros H. rewrite every_reachable_iff in H; destruct H as [H1 H2].
+    split; [apply H2|]. eexists; split; [|right; reflexivity]. apply H1, Hread.
+  }
+  match goal with [ |- ?G ] => assert (Hid : step_r st rid = st -> G) end.
+  {
+    intros Heq; rewrite Heq in *. apply Hsame. intros ? ? ? ?; assumption.
+  }
+  unfold step_r in *.
+  inversion Hread; subst.
+  - rewrite H0 in *; simpl in *.
+    inversion H1; subst.
+    + rewrite H3 in *. destruct is_finished eqn:Hfinished; [|apply Hid; reflexivity].
+      and_left.
+      * eapply unchanged_from_plus_update in Hread.
+        eapply every_reachable_plus_impl; [|rewrite <- unchanged_from_plus_every_reachable; apply Hread].
+        intros a2 Ha2 Heq t Ht; eapply read_addr_same; [eassumption|].
+        eapply unchanged_from_plus_
+        Search unchanged_from_plus. every_reachable_plus. Check unchanged_from_plus_every_reachable. apply <- unchanged_from_plus_every_reachable.
+      intros a Ha t Ht.
+      Search read_addr.
+      eapply read_thread_val.
+      * eapply nth_error_update; eassumption.
+      * unfold is_finished in Hfinished.
+        inversion H4; subst; rewrite H5 in Hfinished; simpl in *; [|congruence].
+        inversion H7; simpl in *; subst; simpl in *; try congruence.
+        injection Hfinished as Hfinished; subst.
+        eapply read_addr_same; [eassumption|].
+        eapply unchanged_from_cycle; [|eassumption].
+        eapply plus_S; [|eapply plus_S; [|apply plus_1]].
+        -- simpl. rewrite H0. left. constructor.
+        -- simpl. rewrite H3. constructor.
+        -- simpl. rewrite H5. left. constructor.
+      * eapply read_cont_same; [eassumption|].
+        intros; eapply read_addr_same; [eassumption|].
+        eapply unchanged_from_cycle; [|eassumption].
+        apply plus_1. simpl. rewrite H0. right. assumption.
+    + rewrite H3.
+      inversion H2; subst; try (eexists; split; [eassumption|right; reflexivity]).
+      eexists; split; [|left; rewrite fill_compose; simpl; apply beta_hnf_ctx, beta_hnf_red, beta_red_lam].
+      unfold subst1, lift_subst. rewrite subst_subst.
+      erewrite subst_ext; [eapply read_thread_term|].
+      * eapply nth_error_update; eassumption.
+      * constructor.
+        -- eapply read_addr_same; [eassumption|].
+           eapply unchanged_from_cycle; [|eassumption].
+           apply plus_1. simpl. rewrite H0. right. constructor.
+        -- eapply read_addr_same_Forall2; [eassumption|].
+           intros; eapply unchanged_from_cycle; [|eassumption].
+           eapply plus_S; [simpl; rewrite H0; left; constructor|].
+           apply plus_1. simpl. rewrite H3. apply clos_points_to_1. assumption.
+      * eapply read_cont_same; [eassumption|].
+        intros; eapply read_addr_same; [eassumption|].
+        eapply unchanged_from_cycle; [|eassumption].
+        apply plus_1. simpl. rewrite H0. right. constructor. assumption.
+      * intros [|n]; unfold comp; simpl; [rewrite read_env_0; reflexivity|].
+        rewrite read_env_S. rewrite subst_ren.
+        erewrite subst_ext; [apply subst_id|].
+        intros n2; unfold comp; simpl. destruct n2; reflexivity.
+    + rewrite H3.
+      admit.
+  - rewrite H0; cbv beta delta [rt_code] iota.
+    destruct t0; cbv iota.
+    + eexists; split; [|right; reflexivity].
+      destruct (nth_error e n) eqn:He; [|assumption].
+      econstructor.
+      * eapply nth_error_update; eassumption.
+      * simpl.
+        eapply nth_error_Forall2 in H1; [|eassumption].
+        destruct H1 as (vv & Hvv1 & Hvv2).
+        eapply read_addr_same; [unfold read_env; rewrite Hvv1; eassumption|].
+        eapply unchanged_from_cycle; [|eassumption].
+        apply plus_1. simpl. rewrite H0. left. constructor. simpl.
+        eapply nth_error_In; eassumption.
+      * eapply read_cont_same; [eassumption|].
+        intros; eapply read_addr_same; [eassumption|].
+        eapply unchanged_from_cycle; [|eassumption].
+        apply plus_1. simpl. rewrite H0. right. assumption.
+    + admit.
+    + destruct c.
+      * eexists; split; [|right; reflexivity]. cbv beta delta [rt_cont] iota.
+        match goal with [ |- read_addr ?st _ _ ] => set (st5 := st) end.
+        match eval unfold st5 in st5 with exit_rthread ?st _ _ => set (st4 := st) end; fold st4 in st5.
+        match eval unfold st4 in st4 with fst (addval ?st _) => set (st3 := st) end; fold st3 in st4, st5.
+        match eval unfold st3 in st3 with fst (makelazy ?st _ _) => set (st2 := st) end; fold st2 in st3, st4, st5.
+        assert (Hchange2 : unchanged_from st st2 (a_rthread rid)) by (eapply unchanged_from_addval; eassumption).
+        assert (Hchange3 : unchanged_from st2 st3 (a_rthread rid)) by (eapply unchanged_from_makelazy, read_addr_same; eassumption).
+        assert (Hchange13 : unchanged_from st st3 (a_rthread rid)) by (eapply unchanged_from_trans; eassumption).
+        assert (Hchange4 : unchanged_from st3 st4 (a_rthread rid)) by (eapply unchanged_from_addval, read_addr_same; eassumption).
+        assert (Hchange14 : unchanged_from st st4 (a_rthread rid)) by (eapply unchanged_from_trans; eassumption).
+        assert (Hchange5 : unchanged_from_plus st4 st5 (a_rthread rid)) by (eapply unchanged_from_plus_update, read_addr_same; eassumption).
+        assert (Hchange15 : unchanged_from_plus st st5 (a_rthread rid)) by (eapply unchanged_from_plus_trans; eassumption).
+        simpl. eapply read_thread_val.
+        -- eapply nth_error_update, nth_error_app_Some; eassumption.
+        -- eapply read_val_clos; [apply nth_error_extend| | |].
+           ++ eapply read_addr_same_Forall2; [eassumption|].
+             intros vp Hvp; apply Hchange15; simpl.
+             rewrite H0; simpl. left; constructor. assumption.
+           ++ eapply read_val_thread; [apply nth_error_app_Some, nth_error_extend|].
+             eapply read_thread_term.
+             ** unfold st5, exit_rthread; simpl; rewrite nth_error_update3; [apply nth_error_extend|].
+                apply nth_error_Some3 in H0; lia.
+             ** constructor.
+                --- eapply read_val_neutral; [apply nth_error_app_Some, nth_error_app_Some, nth_error_extend|].
+                    constructor.
+                --- eapply read_addr_same_Forall2; [eassumption|].
+                    intros vp Hvp; apply Hchange15; simpl.
+                    rewrite H0; simpl. left; constructor. assumption.
+             ** constructor.
+           ++ simpl. apply star_refl.
+        -- inversion H2; subst. constructor.
+      * inversion H2; subst; simpl in *.
+        eexists; split; [|left; rewrite fill_compose; simpl; apply beta_hnf_ctx, beta_hnf_red, beta_red_lam].
+        unfold subst1, lift_subst. rewrite subst_subst.
+        erewrite subst_ext; [eapply read_thread_term|].
+        -- eapply nth_error_update; eassumption.
+        -- constructor.
+           ++ eapply read_addr_same; [eassumption|].
+             eapply unchanged_from_cycle; [|eassumption].
+             apply plus_1. simpl. rewrite H0. right.
+             constructor.
+           ++ eapply read_addr_same_Forall2; [eassumption|].
+             intros; eapply unchanged_from_cycle; [|eassumption].
+             apply plus_1. simpl. rewrite H0. left. constructor. assumption.
+        -- eapply read_cont_same; [eassumption|].
+           intros; eapply read_addr_same; [eassumption|].
+           eapply unchanged_from_cycle; [|eassumption].
+           apply plus_1. simpl. rewrite H0. right. constructor. assumption.
+        -- intros [|n]; unfold comp; simpl; [rewrite read_env_0; reflexivity|].
+           rewrite read_env_S. rewrite subst_ren.
+           erewrite subst_ext; [apply subst_id|].
+           intros n2; unfold comp; simpl. destruct n2; reflexivity.
+      * simpl.
+        eexists; split; [eassumption|right; reflexivity].
+    + eexists. split.
+      * match goal with [ |- read_addr ?st _ _ ] => pose (st2 := st) end.
+        assert (Hchange : unchanged_from_plus st st2 (a_rthread rid)).
+        {
+          eapply unchanged_from_plus_trans; [|eapply unchanged_from_plus_update, read_addr_same; [eassumption|]];
+            eapply unchanged_from_makelazy; eassumption.
+        }
+        eapply read_thread_term; [eapply nth_error_update, nth_error_app_Some; eassumption| |].
+        -- eapply read_addr_same_Forall2; [eassumption|].
+           intros; apply Hchange. simpl; rewrite H0.
+           left. constructor. assumption.
+        -- constructor.
+           ++ eapply read_val_thread; simpl; [rewrite nth_error_extend; reflexivity|].
+             eapply read_thread_term; simpl.
+             ** rewrite nth_error_update3 by (apply nth_error_Some3 in H0; lia).
+                apply nth_error_extend.
+             ** eapply read_addr_same_Forall2; [eassumption|].
+                intros; apply Hchange. simpl; rewrite H0.
+                left. constructor. assumption.
+             ** constructor.
+           ++ eapply read_cont_same; [eassumption|].
+             intros; eapply read_addr_same; [eassumption|].
+             apply Hchange. simpl; rewrite H0.
+             right. assumption.
+      * right. rewrite fill_compose. reflexivity.
+    + admit.
+    + admit.
+Admitted.
+
+Lemma stable_beta_hnf :
+  forall st st2 rid t t2,
+    read_addr st (a_rthread rid) t ->
+    read_addr st2 (a_rthread rid) t2 ->
+    unchanged_from_plus st st2 (a_rthread rid) ->
+    reflc beta_hnf t t2 ->
+    stable st st2 (a_rthread rid) ->
+    (forall a t3, read_addr st a t3 -> exists t4, read_addr st2 a t4 /\ star beta_hnf t3 t4).
+Proof.
+  intros st st2 rid t t2 Hread1 Hread2 Hchange Hreflc (_ & Hdel & Hstable) a t3 Hread.
+  assert (Hacc := read_addr_Acc _ _ _ Hread). induction Hacc.
+  destruct (proj2 (Hstable x)) as [Heq | [[Hnone | Hstar] Hpoints]].
+  - admit.
+  - inversion Hread; subst; simpl in *; congruence.
+  inversion Hread; subst.
+  - 
+  Search Acc.
+  induction Hread.
